# Final Exam Notes

## Fractions 
#### Adding by finding LCD
$\dfrac{1}{4} + \dfrac{1}{2} => \dfrac{1}{4} + \dfrac{1(2)}{2(2)} =>\dfrac{1}{4} + \dfrac{2}{4} = \dfrac{3}{4}$

#### Adding/Subtracing by finding common denominator
$\dfrac{1}{5} + \dfrac{1}{2} => \dfrac{1(2)}{5(2)} + \dfrac{1(5)}{2(5)} => \dfrac{2}{10} + \dfrac{5}{10} = \dfrac{7}{10}$

#### Multiplying Fractions by multiplying straight across
$\dfrac{1}{2} * \dfrac{1}{2} => \dfrac{1(1)}{2(2)} = \dfrac{1}{4}$

#### Dividing Fractions by reciprical
$\dfrac{1}{2} \div \dfrac{1}{3} => \dfrac{1}{2} \times \dfrac{3}{1} = \dfrac{3}{2}$

## Decimals
#### Adding Decimanls
$6.56 + 3.29$   
&nbsp;&nbsp;&nbsp;$6.56$  
$+3.29$   
$====$  
&nbsp;&nbsp;&nbsp;&nbsp;&nbsp;&nbsp;$1$  
&nbsp;&nbsp;&nbsp;$6.56$  
$+3.29$  
$====$   
&nbsp;&nbsp;&nbsp;$9.85$

## Formulas
### Quadratic Formula
$\dfrac{-b \pm \sqrt{b^2-4(a)(c)}}{2(a)}$

### Point Slope
$y-y_1 = m(x-x_1)$

### Slope Intercept Form
$y=mx+b$

### Standard Form
$a+by=c$

### Slope Form
$m = \dfrac{y_2 - y_1}{x_2 - x_1}$

### Vertex of a parabola
$x = -\dfrac{b}{2a}$<br>
$y = ax^2+bx+c$ where x is the value above.

### Circle Midpoint
$m = (\dfrac{x_1+x_2}{2}, \dfrac{y_1+y_2}{2})$

### Interest (Compound)
$A = P(1+\frac{r}{n})^{nt}$

### Interest (Contin.)
$P(t) = P_0e^{rt}$

## Properties of Exponents
Product: $x^n * x^m = x^{n+m}$<br>
Power: $(x^n)^m = x^{n*m}$<br>
Quotient: $\dfrac{x^n}{x^m} = x^{n-m}$<br>
Dist. of Products: $(x * y)^n = x^n * y^n$<br>
Dist. of Quotients: $(\dfrac{x}{y})^n = \dfrac{x^n}{y^n}$<br>
Negatives: $x^{-n} = \dfrac{1}{x^n}$

## Radicals
Radicals to exponents: <br>$\sqrt{a} = a^{1/2}$<br>
$\sqrt[m]{a} = a^{1/m}$<br>
$\sqrt[m]{a^n} = a^{n/m}$<br>

## Dividing Polynomials
$(\dfrac{x^2y^6z^4}{x^-2y^-6z^-4})^{-2}$<br>
Using the Quotient Property of Exponents<br>
$(x^{2-(-2)}y^{6-(-6)}z^{4-(-4)})^{-2}$<br>
$(x^4y^{12}z^8)^{-2}$<br> Using the negatives<br>
$(x^4)^{-2}(y^{12})^{-2}(z^8)^{-2}$ = $\dfrac{1}{x^8y^{24}z^{16}}$

## Polynomials with Negative Exponents
Solve by substitution<br>
$2x^{-2}-13x^{-1} +20 = 0$<br>
Where $u = x^{-1}$<br>
$2u^2-13u+20 = 0$<br>
$(2u-5)(u-4)$<br>
$(2u-5) = 0$&nbsp;&nbsp;$(u-4) = 0$<br>
$u = \dfrac{5}{2}$&nbsp;&nbsp;$u = 4$<br>
$x^{-1} = \dfrac{5}{2}$&nbsp;&nbsp;$x^{-1} = 4$<br>
$(x^{-1})^{-1} = (\dfrac{5}{2})^{-1}$&nbsp;&nbsp;$(x^{-1})^{-1} = (4)^{-1}$<br>
$x= \dfrac{2}{5}$&nbsp;&nbsp;$x = \dfrac{1}{4}$<br>

## Properties of Logarithms
Log of 1: $\log_a1=0$<br>
Log of base match: $\log_a a =1$<br>
Product: $\log_a(mn) = \log_a m + \log_a n$<br>
Quotient: $\log_a\dfrac{m}{n} = \log_a m - \log_a n$<br>
Power: $\log_a m^n = n*\log_a m$<br>
Change of Base: $\log_b a = \dfrac{\log_ca}{\log_cb}$<br>
Equality: $\log_b a = \log_b c => a = c$<br>
Number Raised to Log: $a^{\log_ax} = x$<br>
Negative: $-\log_b a = \log_b \dfrac{1}{a}$<br>

## Natural Logarithms
$\ln 1 = 0$<br>
$\ln e = 1$<br>
$\ln(mn) = \ln m + \ln n$<br>
$\ln m^n = n \ln m$<br>
$e^{\ln x} = x$

## Inequalities
When mul/div by negative flip sign.

## Zeros of Polynomials
When factorable factor and solve when equation is set to zero<br>

When not factorable use synthetic division (by the factors of the leading coefficient and the constant) if there is no remainder than it is a zero. 

## Asymptotes
Finding a Vertical Asymptote:<br>
We can find vertical asymptotes by simply equating the denominator to zero and then solving for x<br><br>
Finding a Horizontal Asymptote:<br>
Put the rational function in a standard form. That is, expand the numerator and denominator if they are written in a factored form.

Remove all terms except the terms that contain the largest exponents of x in the numerator and the denominator.

There are three possibilities:

        If the degree of the numerator is smaller than the degree of the denominator, then the horizontal asymptote crosses the x-axis at . That is, it is the x-axis itself.
        If the degree of the denominator and the numerator are the same, then the horizontal asymptote equals to the ratio of the leading coefficients.
        If the degree of the numerator is larger than the degree of the denominator, then there is no horizontal asymptote.

## Composition of functions
$(f ยบ g)(x) = f(g(x))$

## Algebra of functions
$(f+g)(x) = f(x) + g(x)$ and so on.<br>
Example:<br>
$(x^2+2) + (x^2 +3) = x^2 +2 + x^2 + 3 = 2x^2 +5$<br>

## Rationalizing the Denom.
Multiply by conjugate.<br>
Example:<br>
$3 - \sqrt{10}$ becomes $3 + \sqrt{10}$